ulib/FStar.TSet.fst
@@ -134,5 +134,36 @@ private let lemma_mem_tset_of_set_r (#a:eqtype) (s:Set.set a) (x:a)
 let lemma_mem_tset_of_set (#a:eqtype) (s:Set.set a) (x:a)
   :Lemma (requires True)
          (ensures  (Set.mem x s <==> mem x (tset_of_set s)))
-	 [SMTPat (mem x (tset_of_set s))]
+         [SMTPat (mem x (tset_of_set s))]
   = lemma_mem_tset_of_set_l #a s x; lemma_mem_tset_of_set_r #a s x
+
+abstract
+let filter (#a:Type) (f:a -> Type0) (s:set a) : set a =
+  (fun (x:a) -> f x /\ s x)
+
+let lemma_mem_filter (#a:Type) (f:(a -> Type0)) (s:set a) (x:a)
+  :Lemma (requires True)
+         (ensures  (mem x (filter f s) <==> mem x s /\ f x))
+         [SMTPat (mem x (filter f s))]
+  = ()
+
+let exists_y_in_s (#a:Type) (#b:Type) (s:set a) (f:a -> b) (x:b) : prop =
+ exists (y:a). mem y s /\ x == f y
+
+abstract
+let map (#a:Type) (#b:Type) (f:a -> b) (s:set a) : set b = exists_y_in_s s f
+
+let lemma_mem_map (#a:Type) (#b:Type) (f:(a -> b)) (s:set a) (x:b)
+  :Lemma ((exists (y:a). {:pattern (mem y s)} mem y s /\ x == f y) <==> mem x (map f s))
+         [SMTPat (mem x (map f s))]
+  = ()
+
+(* TODO: For some reason, this definition does not typecheck here *)
+(* val as_set': #a:Type -> list a -> Tot (set a) *)
+(* let rec as_set' #a l =  *)
+(*   match l with *)
+(*   | [] -> admit() *)
+(*   | hd::tl -> admit() *)
+
+(* unfold val as_set:  #a:Type -> l:list a -> Tot (set a) *)
+(* let as_set (#a:Type) (l:list a) = normalize_term (as_set' l) *)
